

Homework Sheet 6

Author: Abdullah Oğuz Topçuoğlu

Exercise 21

We are given the function

$$f(x_1, x_2) := \begin{pmatrix} \log(1 + x_1^2 + 2x_2^2) \\ x_1 e^{2x_2} \end{pmatrix}.$$

(i)

The jacobian matrix is invertible at the points where the determinant is not zero.

The jacobian matrix:

$$J_f(x_1, x_2) = \begin{pmatrix} \frac{2x_1}{1+x_1^2+2x_2^2} & \frac{4x_2}{1+x_1^2+2x_2^2} \\ e^{2x_2} & 2x_1 e^{2x_2} \end{pmatrix}.$$

The determinant of the jacobian matrix:

$$\begin{aligned} \det(J_f(x_1, x_2)) &= \frac{2x_1 \cdot 2x_1 e^{2x_2}}{1 + x_1^2 + 2x_2^2} - \frac{4x_2 \cdot e^{2x_2}}{1 + x_1^2 + 2x_2^2} \\ &= \frac{4x_1^2 e^{2x_2} - 4x_2 e^{2x_2}}{1 + x_1^2 + 2x_2^2} \\ &= \frac{4e^{2x_2}(x_1^2 - x_2)}{1 + x_1^2 + 2x_2^2}. \end{aligned}$$

The determinant is zero when

$$4e^{2x_2}(x_1^2 - x_2) = 0 \implies x_1^2 - x_2 = 0 \implies x_2 = x_1^2.$$

The set A would be

$$A = \{(x_1, x_2) \in \mathbb{R}^2 : x_2 \neq x_1^2\}.$$

(ii)

f is locally invertible at a point if the jacobian matrix is invertible at that point and we know that the jacobian matrix is invertible at each point in A .

So f is locally invertible at each point $x \in A$.

(iii)

To find the jacobian matrix of the local inverse of f at $f(x)$, we can use the formula:

$$J_{f^{-1}}(f(x)) = (J_f(x))^{-1}.$$

We already have $J_f(x)$ so we need to find its inverse.
The jacobian matrix:

$$J_f(x_1, x_2) = \begin{pmatrix} \frac{2x_1}{1+x_1^2+2x_2^2} & \frac{4x_2}{1+x_1^2+2x_2^2} \\ e^{2x_2} & 2x_1 e^{2x_2} \end{pmatrix}.$$

And its determinant:

$$\det(J_f(x_1, x_2)) = \frac{4e^{2x_2}(x_1^2 - x_2)}{1 + x_1^2 + 2x_2^2}.$$

We calculated those in the previous parts.
The inverse of jacobian matrix:

$$\begin{aligned} (J_f(x_1, x_2))^{-1} &= \frac{1}{\det(J_f(x_1, x_2))} \begin{pmatrix} 2x_1 e^{2x_2} & -\frac{4x_2}{1+x_1^2+2x_2^2} \\ -e^{2x_2} & \frac{2x_1}{1+x_1^2+2x_2^2} \end{pmatrix} \\ &= \frac{1 + x_1^2 + 2x_2^2}{4e^{2x_2}(x_1^2 - x_2)} \begin{pmatrix} 2x_1 e^{2x_2} & -\frac{4x_2}{1+x_1^2+2x_2^2} \\ -e^{2x_2} & \frac{2x_1}{1+x_1^2+2x_2^2} \end{pmatrix} \end{aligned}$$

Exercise 22

(i)

We are given the integral

$$\int_A \frac{1}{x_1^3} + \frac{2}{x_2^2} d(x_1, x_2)$$

where $A = [1, 3] \times [2, 4]$.

The function $\frac{1}{x_1^3} + \frac{2}{x_2^2}$ is continuous on the set A because it is obviously a C^1 function which implies continuity. It is a C^1 function because all the partial derivatives exist and are continuous.

And continuity of the integrand implies integrability therefore the integral exists.

Since it is integrable we can use the Fubini theorem

$$\begin{aligned}
\int_A \frac{1}{x_1^3} + \frac{2}{x_2^2} d(x_1, x_2) &= \int_1^3 \int_2^4 \left(\frac{1}{x_1^3} + \frac{2}{x_2^2} \right) dx_2 dx_1 \\
&= \int_1^3 \left(\int_2^4 \frac{1}{x_1^3} dx_2 + \int_2^4 \frac{2}{x_2^2} dx_2 \right) dx_1 \\
&= \int_1^3 \left(\frac{1}{x_1^3} (4 - 2) + 2 \left(-\frac{1}{x_2} \Big|_2^4 \right) \right) dx_1 \\
&= \int_1^3 \left(\frac{2}{x_1^3} + 2 \left(-\frac{1}{4} + \frac{1}{2} \right) \right) dx_1 \\
&= \int_1^3 \left(\frac{2}{x_1^3} + 2 \left(\frac{1}{4} \right) \right) dx_1 \\
&= \int_1^3 \left(\frac{2}{x_1^3} + \frac{1}{2} \right) dx_1 \\
&= 2 \left(-\frac{1}{2x_1^2} \Big|_1^3 \right) + \frac{1}{2} (3 - 1) \\
&= 2 \left(-\frac{1}{18} + \frac{1}{2} \right) + 1 \\
&= 2 \left(\frac{9 - 1}{18} \right) + 1 = 2 \left(\frac{8}{18} \right) + 1 = \frac{8}{9} + 1 = \frac{17}{9}.
\end{aligned}$$

(ii)

We are given the integral

$$\int_A \cos(x_1) x_2^3 d(x_1, x_2)$$

where $A = \left[-\frac{\sqrt{\pi}}{2}, \frac{\sqrt{\pi}}{2} \right] \times [-1, 1]$.

The function $\cos(x_1) x_2^3$ is continuous on the set A because it is obviously a C^1 function which implies continuity. It is a C^1 function because all the partial derivatives exist and are continuous.

And continuity of the integrand implies integrability therefore the integral exists.

Since it is integrable we can use the Fubini theorem

$$\begin{aligned}
\int_A \cos(x_1) x_2^3 d(x_1, x_2) &= \int_{-\frac{\sqrt{\pi}}{2}}^{\frac{\sqrt{\pi}}{2}} \int_{-1}^1 \cos(x_1) x_2^3 dx_2 dx_1 \\
&= \int_{-\frac{\sqrt{\pi}}{2}}^{\frac{\sqrt{\pi}}{2}} \cos(x_1) \left(\int_{-1}^1 x_2^3 dx_2 \right) dx_1 \\
&= \int_{-\frac{\sqrt{\pi}}{2}}^{\frac{\sqrt{\pi}}{2}} \cos(x_1) \left(\frac{x_2^4}{4} \Big|_{-1}^1 \right) dx_1 \\
&= \int_{-\frac{\sqrt{\pi}}{2}}^{\frac{\sqrt{\pi}}{2}} \cos(x_1) \left(\frac{1}{4} - \frac{1}{4} \right) dx_1 \\
&= \int_{-\frac{\sqrt{\pi}}{2}}^{\frac{\sqrt{\pi}}{2}} \cos(x_1) \cdot 0 dx_1 = 0.
\end{aligned}$$